moving stuff

thy/Bitmagic/Numberwang_Ln.thy
@@ -10,25 +10,62 @@ apply(simp add: ipv4set_from_cidr_eq_ip_cidr_set)
 using ip_cidr_set_notsubset_empty_inter by blast
 
 
-(*
-lemma help1: "word_of_int (uint a mod 256) = a mod (256::ipv4addr)"
-by(simp add: word_mod_def)
-lemma help2: "nat_of_ipv4addr ((ip::ipv4addr) AND mask 8) = (nat_of_ipv4addr ip) mod 256"
-  apply(simp add: nat_of_ipv4addr_def)
-  apply(simp add: and_mask_mod_2p)
-  apply(simp add: help1)
-  apply(simp add: unat_mod)
+
+fun ipcidr_conjunct :: "('i::len word \<times> nat) \<Rightarrow> ('i word \<times> nat) \<Rightarrow> ('i word \<times> nat) option" where 
+  "ipcidr_conjunct (base1, m1) (base2, m2) = (if ipset_from_cidr base1 m1 \<inter> ipset_from_cidr base2 m2 = {}
+     then
+      None
+     else if 
+      ipset_from_cidr base1 m1 \<subseteq> ipset_from_cidr base2 m2
+     then 
+      Some (base1, m1)
+     else
+      Some (base2, m2)
+    )"
+
+lemma ipcidr_conjunct_any: "ipcidr_conjunct (0, 0) (0, 0) \<noteq> None"
+  by(simp add: ipset_from_cidr_0)
+
+lemma ipcidr_conjunct_correct: "(case ipcidr_conjunct (b1, m1) (b2, m2)
+                                        of Some (bx, mx) \<Rightarrow> ipset_from_cidr bx mx
+                                        |  None \<Rightarrow> {})
+    = (ipset_from_cidr b1 m1) \<inter> (ipset_from_cidr b2 m2)"
+  apply(simp split: split_if_asm)
+  using ip_cidr_intersect by fast
+declare ipcidr_conjunct.simps[simp del]
+
+
+  (*TODO: this is a duplicate, right?*)
+  (*TODO: if not, move!*)
+  definition ipcidr_tuple_to_wordinterval :: "('i::len word \<times> nat) \<Rightarrow> 'i wordinterval" where
+    "ipcidr_tuple_to_wordinterval iprng = iprange_interval (ipcidr_to_interval iprng)"
+
+  
+  (*TODO: rename*)
+  lemma wordinterval_to_set_ipcidr_tuple_to_wordinterval:
+    "wordinterval_to_set (ipcidr_tuple_to_wordinterval (b, m)) = ipset_from_cidr b m"
+    unfolding ipcidr_tuple_to_wordinterval_def ipset_from_cidr_ipcidr_to_interval ipcidr_to_interval_def
+    by(simp add: iprange_interval.simps)
+
+
+  lemma [code_unfold]: 
+  "ipcidr_conjunct ips1 ips2 = (if wordinterval_empty (wordinterval_intersection (ipcidr_tuple_to_wordinterval ips1) (ipcidr_tuple_to_wordinterval ips2))
+       then
+        None
+       else if 
+        wordinterval_subset (ipcidr_tuple_to_wordinterval ips1) (ipcidr_tuple_to_wordinterval ips2)
+       then 
+        Some ips1
+       else
+        Some ips2
+      )"
+  apply(simp)
+  apply(cases ips1, cases ips2, rename_tac b1 m1 b2 m2, simp)
+  apply(safe)
+     apply(auto simp add: wordinterval_to_set_ipcidr_tuple_to_wordinterval ipcidr_conjunct.simps split:split_if_asm)
   done
-lemma help3: "(nat_of_ipv4addr ip mod 256) = (nat_of_ipv4addr (ip mod 256))"
-  by(simp add: nat_of_ipv4addr_def unat_mod)
-
-lemma ip_shiftr_div_consts: "(ip::ipv4addr) >> 24 = ip div (2^24)"
-      "(ip::ipv4addr) >> 16 = ip div (2^16)"
-      "(ip::ipv4addr) >> 8 = ip div (2^8)"
-by(subst Word.word_uint_eq_iff, simp add: shiftr_div_2n uint_div)+
-*)
-
-
+  (*with the code_unfold lemma before, this works!*)
+  lemma "ipcidr_conjunct (0::32 word,0) (8,1) = Some (8, 1)" by eval
 
 
 
